
\chapter{Conditional distribution of $\beta_0$} \label{beta0}

Here, it will be shown that $\beta_0$ conditionally has the von Mises distribution, that is
\begin{equation}
L(\beta_0 \mid \kappa, \bdt, \bbt, \bt, \bX, \bd)  \propto \mathcal{VM}(\beta_0 \mid \bar\psi, R_{\psi}\kappa).
\end{equation} %\propto \exp \left\lbrace \kappa \sum_{i=1}^n \cos \left[ \theta_i - (\beta_0 + g(\boldsymbol\beta^T \boldsymbol{x}_i)) \right]  \right\rbrace
The proof for the conditional distribution of $\beta_0$ in the GLM closely follows the derivation for the distribution of the mean direction $\mu$ of the von Mises distribution, which shows that $L(\mu \mid \kappa, \boldsymbol\theta) \propto \mathcal{VM}(\mu \mid \bar\theta, R_{\theta} \kappa)$.

The conditional likelihood of $\beta_0$ is given by

\begin{align*}
L(\beta_0 \mid \kappa, \bdt, \bbt, \bt, \bX, \bd) & \propto \exp \left\lbrace \kappa \sum_{i=1}^n \cos \left[ \theta_i - (\beta_0 + \bdt^T \bd_i +  g(\boldsymbol\beta^T \boldsymbol{x}_i)) \right] \right\rbrace \\
& = \exp \left\lbrace \kappa \sum_{i=1}^n \cos \left[ \beta_0 - (\theta_i - \bdt^T \bd_i - g(\boldsymbol\beta^T \boldsymbol{x}_i)) \right]  \right\rbrace.
\end{align*}

We know that for any angle $\psi_i, i = 1, \dots, n$,

\begin{equation*}
 C_{\psi} = \sum_{i=1}^n \cos(\psi_i), ~~ S_{\psi} = \sum_{i=1}^n \sin(\psi_i), ~~ R_{\psi} = \sqrt{C_{\psi}^2 + S_{\psi}^2}, ~~
\end{equation*}
\begin{equation*}
 \text{and} ~~ \frac{C_{\psi}}{R_{\psi}} = \cos \bar\psi, ~~ \frac{S_{\psi}}{R_{\psi}} = \sin \bar\psi, ~~ \text{where} ~~ \bar\psi = \atantwo(S_{\psi}, C_{\psi}).
\end{equation*}

Thus, setting angle $\psi_i = \theta_i - \bdt^T \bd_i - g(\boldsymbol\beta^T \boldsymbol{x}_i)$,


\begin{align*}
L(\beta_0 \mid \kappa, \bdt, \bbt, \bt, \bX, \bd) & \propto \exp \left\lbrace \kappa \sum_{i=1}^n \cos ( \beta_0 - \psi_i)  \right\rbrace \\
& = \exp \left\lbrace \kappa   \left[ \cos\beta_0 \sum_{i=1}^n \cos\psi_i +  \sin\beta_0 \sum_{i=1}^n \sin\psi_i \right]  \right\rbrace \\
& = \exp \left\lbrace R_{\psi}  \kappa  \left[ \cos\beta_0 \frac{C_{\psi}}{R_{\psi}} +  \sin\beta_0 \frac{S_{\psi}}{R_{\psi}} \right]  \right\rbrace \\
& = \exp \left\lbrace R_{\psi} \kappa   \left[ \cos\beta_0 \cos{\bar\psi} +  \sin\beta_0 \sin{\bar\psi}\right]  \right\rbrace \\
& = \exp \left\lbrace R_{\psi} \kappa \cos \left( \beta_0 - \bar\psi \right)  \right\rbrace \\
& \propto \mathcal{VM}(\beta_0 \mid \bar\psi, R_{\psi} \kappa).
\end{align*}









